examples/cms/verif_CMS_insert.v
@@ -1,0 +1,349 @@
+Require Import Poulet4.P4light.Syntax.P4defs.
+Require Import Poulet4.P4light.Semantics.Semantics.
+Require Import ProD3.core.Core.
+Require Import ProD3.core.Tofino.
+Require Import ProD3.examples.cms.ConModel.
+Require Import ProD3.examples.cms.common.
+Require Import ProD3.examples.cms.ModelRepr.
+Require Import ProD3.examples.cms.verif_Win1.
+Require Import ProD3.examples.cms.verif_Win2.
+Require Import ProD3.examples.cms.verif_Win3.
+Require Import ProD3.examples.cms.verif_CMS_1.
+
+#[local] Hint Extern 5 (func_modifies _ _ _ _ _) => (apply tbl_hash_index_1_body) : func_specs.
+#[local] Hint Extern 5 (func_modifies _ _ _ _ _) => (apply tbl_hash_index_2_body) : func_specs.
+#[local] Hint Extern 5 (func_modifies _ _ _ _ _) => (apply tbl_hash_index_3_body) : func_specs.
+#[local] Hint Extern 5 (func_modifies _ _ _ _ _) => (apply tbl_hash_index_4_body) : func_specs.
+#[local] Hint Extern 5 (func_modifies _ _ _ _ _) => (apply tbl_hash_index_5_body) : func_specs.
+#[local] Hint Extern 5 (func_modifies _ _ _ _ _) => (apply tbl_clear_index_body) : func_specs.
+#[local] Hint Extern 5 (func_modifies _ _ _ _ _) => (apply tbl_clear_window_body) : func_specs.
+#[local] Hint Extern 5 (func_modifies _ _ _ _ _) => (apply act_set_clear_win_1_body) : func_specs.
+#[local] Hint Extern 5 (func_modifies _ _ _ _ _) => (apply act_set_clear_win_2_body) : func_specs.
+#[local] Hint Extern 5 (func_modifies _ _ _ _ _) => (apply act_set_clear_win_3_body) : func_specs.
+
+Definition P4_bf2_win_md_t_insert (f cf if' : Z) (new_clear_index : Sval) (is : list Sval) :=
+  if f=? cf then
+    P4_bf2_win_md_t (P4Bit 8 CLEAR) (Zrepeat new_clear_index 5)
+  else if f=? if' then
+    P4_bf2_win_md_t (P4Bit 8 INSERT) is
+  else
+    P4_bf2_win_md_t (P4Bit 8 NOOP) is.
+
+Definition tbl_set_win_insert_spec : func_spec :=
+  WITH (* p *),
+    PATH p
+    MOD (Some [["ds_md"];
+               ["act_set_clear_win_1"; "api_1"];
+               ["act_set_clear_win_1"; "api_2"];
+               ["act_set_clear_win_1"; "api_3"];
+               ["act_set_clear_win_2"; "api_1"];
+               ["act_set_clear_win_2"; "api_2"];
+               ["act_set_clear_win_2"; "api_3"];
+               ["act_set_clear_win_3"; "api_1"];
+               ["act_set_clear_win_3"; "api_2"];
+               ["act_set_clear_win_3"; "api_3"];
+               ["act_set_clear_win_4"; "api_1"];
+               ["act_set_clear_win_4"; "api_2"];
+               ["act_set_clear_win_4"; "api_3"];
+               ["act_set_clear_win_5"; "api_1"];
+               ["act_set_clear_win_5"; "api_2"];
+               ["act_set_clear_win_5"; "api_3"]]) []
+    WITH (timer : Z * bool) (clear_index_1 hash_index_1 hash_index_2 hash_index_3 hash_index_4 hash_index_5 : Sval)
+      (H_timer : 0 <= fst timer < frame_tick_tocks * num_frames),
+      PRE
+        (ARG []
+        (MEM [(["api"], P4Bit 8 INSERT);
+              (["ds_md"], ValBaseStruct
+                 [("clear_window", P4Bit 16 (fst timer));
+                  ("clear_index_1", clear_index_1);
+                  ("hash_index_1", hash_index_1);
+                  ("hash_index_2", hash_index_2);
+                  ("hash_index_3", hash_index_3);
+                  ("hash_index_4", hash_index_4);
+                  ("hash_index_5", hash_index_5);
+                  ("win_1", P4_bf2_win_md_t_);
+                  ("win_2", P4_bf2_win_md_t_);
+                  ("win_3", P4_bf2_win_md_t_)])]
+        (EXT [])))
+      POST
+        (EX retv,
+        (ARG_RET [] retv
+        (let cf := get_clear_frame timer in
+        let if' := get_insert_frame cf in
+        (MEM [(["ds_md"], ValBaseStruct
+                 [("clear_window", P4Bit 16 (fst timer));
+                  ("clear_index_1", clear_index_1);
+                  ("hash_index_1", hash_index_1);
+                  ("hash_index_2", hash_index_2);
+                  ("hash_index_3", hash_index_3);
+                  ("hash_index_4", hash_index_4);
+                  ("hash_index_5", hash_index_5);
+                  ("win_1", P4_bf2_win_md_t_insert 0 cf if' clear_index_1
+                        [hash_index_1; hash_index_2; hash_index_3; hash_index_4; hash_index_5]);
+                  ("win_2", P4_bf2_win_md_t_insert 1 cf if' clear_index_1
+                        [hash_index_1; hash_index_2; hash_index_3; hash_index_4; hash_index_5]);
+                  ("win_3", P4_bf2_win_md_t_insert 2 cf if' clear_index_1
+                        [hash_index_1; hash_index_2; hash_index_3; hash_index_4; hash_index_5])])]
+        (EXT [])))))%arg_ret_assr.
+
+Lemma tbl_set_win_insert_body :
+  func_sound ge tbl_set_win_fd nil tbl_set_win_insert_spec.
+Proof.
+  start_function; elim_trivial_cases.
+  - replace (get_clear_frame timer) with 0. 2 : {
+      symmetry; eapply Z_div_squeeze'; eauto.
+    }
+    table_action act_set_clear_win_1_body.
+    { entailer. }
+    { entailer. }
+  - replace (get_clear_frame timer) with 1. 2 : {
+      symmetry; eapply Z_div_squeeze'; eauto.
+    }
+    table_action act_set_clear_win_2_body.
+    { entailer. }
+    { entailer. }
+  - replace (get_clear_frame timer) with 2. 2 : {
+      symmetry; eapply Z_div_squeeze'; eauto.
+    }
+    table_action act_set_clear_win_3_body.
+    { entailer. }
+    { entailer. }
+  - lia.
+Qed.
+
+#[local] Hint Extern 5 (func_modifies _ _ _ _ _) => (apply tbl_set_win_insert_body) : func_specs.
+
+Definition cms_insert := @cms_insert num_frames num_rows num_slots H_num_frames H_num_rows H_num_slots
+  frame_tick_tocks.
+
+Definition CMS_insert_spec : func_spec :=
+  WITH (* p *),
+    PATH p
+    MOD None [p]
+    WITH (key : Val) (tstamp : Z) (cf : cms num_frames num_rows num_slots),
+      PRE
+        (ARG [eval_val_to_sval key; P4Bit 8 INSERT; P4Bit 48 tstamp; P4Bit 8 0]
+        (MEM []
+        (EXT [cms_repr p index_w panes rows cf])))
+      POST
+        (ARG_RET [P4Bit 8 0] ValBaseNull
+        (MEM []
+        (EXT [cms_repr p index_w panes rows (cms_insert cf (Z.odd (tstamp/tick_time)) (hashes key))]))).
+
+Lemma CMS_insert_body :
+  func_sound ge Filter_fd nil CMS_insert_spec.
+Proof.
+  Time start_function.
+  destruct cf as [[ps ?H] ? ?].
+  unfold cms_repr.
+  cbn [proj1_sig] in *.
+  destruct_list ps.
+  normalize_EXT.
+  Time step.
+  Time step_call tbl_hash_index_1_body.
+  { entailer. }
+  Intros _.
+  step_call tbl_hash_index_2_body.
+  { entailer. }
+  Time simpl_assertion.
+  Intros _.
+  step_call tbl_hash_index_3_body.
+  { entailer. }
+  Time simpl_assertion.
+  Intros _.
+  step_call tbl_hash_index_4_body.
+  { entailer. }
+  Time simpl_assertion.
+  Intros _.
+  step_call tbl_hash_index_5_body.
+  { entailer. }
+  Time simpl_assertion.
+  Intros _.
+  set (is := (exist _ [hash1 key; hash2 key; hash3 key; hash4 key; hash5 key] eq_refl : listn Z num_rows)).
+  set (clear_is := (exist _ (Zrepeat cms_clear_index num_rows) eq_refl : listn Z num_rows)).
+  assert (Forall (fun i : Z => 0 <= i < num_slots) (`is)). {
+    repeat first [apply Forall_cons | apply Forall_nil].
+    all : apply Z.mod_pos_bound; lia.
+  }
+  P4assert (0 <= cms_clear_index < num_slots). {
+    unfold fil_clear_index_repr.
+    Intros i'.
+    normalize_EXT.
+    Intros_prop.
+    apply ext_implies_prop_intro.
+    subst.
+    apply Z.mod_pos_bound.
+    lia.
+  }
+  assert (Forall (fun i : Z => 0 <= i < num_slots) (`clear_is)). {
+    repeat first [
+      assumption
+    | constructor
+    ].
+  }
+  step_call tbl_clear_index_body.
+  { entailer. }
+  Time simpl_assertion.
+  Intros _.
+  step_call tbl_clear_window_body.
+  { entailer. }
+  Intros _.
+  set (new_timer := update_timer cms_timer (Z.odd (tstamp / tick_time))).
+  P4assert (0 <= fst new_timer < num_frames * frame_tick_tocks).
+  { unfold timer_repr.
+    normalize_EXT.
+    Intros_prop.
+    apply ext_implies_prop_intro.
+    auto.
+  }
+  step_call tbl_set_win_insert_body.
+  { entailer. }
+  { auto. }
+  Intros _.
+  (* unfold and fold in the post condition *)
+  unfold cms_insert, ConModel.cms_insert.
+  unfold proj1_sig.
+  fold new_timer.
+  replace (exist (fun i : list Z => Zlength i = num_rows) (Zrepeat cms_clear_index num_rows) _) with clear_is. 2 : {
+    apply subset_eq_compat. auto.
+  }
+  assert (0 <= get_clear_frame new_timer < num_frames). {
+    unfold ConModel.get_clear_frame.
+    split.
+    - apply Z.div_le_lower_bound; lia.
+    - apply Z.div_lt_upper_bound; lia.
+  }
+  destruct (get_clear_frame new_timer =? 0) eqn:?.
+  { replace (get_clear_frame new_timer) with 0 by lia.
+    step_call verif_Win1.Win_body _ _ clear_is.
+    { entailer. }
+    { solve [repeat constructor]. }
+    { auto. }
+    step_call verif_Win2.Win_body _ _ is.
+    { entailer. }
+    { solve [repeat constructor]. }
+    { auto. }
+    step_call verif_Win3.Win_body _ _ is.
+    { entailer. }
+    { solve [repeat constructor]. }
+    { auto. }
+    simpl Z.eqb. cbn match.
+    step_call tbl_merge_wins_1_body.
+    { entailer. }
+    { reflexivity. }
+    { reflexivity. }
+    Intros _.
+    simpl_assertion.
+    step_into.
+    { hoare_func_table; elim_trivial_cases.
+      { clear -H5; lia. }
+      table_action NoAction_body.
+      { entailer. }
+      { apply arg_ret_implies_refl. }
+    }
+    { reflexivity. }
+    { reflexivity. }
+    simpl_assertion.
+    entailer.
+  }
+  destruct (get_clear_frame new_timer =? 1) eqn:?.
+  { replace (get_clear_frame new_timer) with 1 by lia.
+    step_call verif_Win1.Win_body _ _ is.
+    { entailer. }
+    { solve [repeat constructor]. }
+    { auto. }
+    step_call verif_Win2.Win_body _ _ clear_is.
+    { entailer. }
+    { solve [repeat constructor]. }
+    { auto. }
+    step_call verif_Win3.Win_body _ _ is.
+    { entailer. }
+    { solve [repeat constructor]. }
+    { auto. }
+    simpl Z.eqb. cbn match.
+    step_call tbl_merge_wins_1_body.
+    { entailer. }
+    { reflexivity. }
+    { reflexivity. }
+    Intros _.
+    simpl_assertion.
+    step_into.
+    { hoare_func_table; elim_trivial_cases.
+      { clear -H5; lia. }
+      table_action NoAction_body.
+      { entailer. }
+      { apply arg_ret_implies_refl. }
+    }
+    { reflexivity. }
+    { reflexivity. }
+    simpl_assertion.
+    entailer.
+  }
+  destruct (get_clear_frame new_timer =? 2) eqn:?.
+  { replace (get_clear_frame new_timer) with 2 by lia.
+    step_call verif_Win1.Win_body _ _ is.
+    { entailer. }
+    { solve [repeat constructor]. }
+    { auto. }
+    step_call verif_Win2.Win_body _ _ is.
+    { entailer. }
+    { solve [repeat constructor]. }
+    { auto. }
+    step_call verif_Win3.Win_body _ _ clear_is.
+    { entailer. }
+    { solve [repeat constructor]. }
+    { auto. }
+    simpl Z.eqb. cbn match.
+    step_call tbl_merge_wins_1_body.
+    { entailer. }
+    { reflexivity. }
+    { reflexivity. }
+    Intros _.
+    simpl_assertion.
+    step_into.
+    { hoare_func_table; elim_trivial_cases.
+      { clear -H5; lia. }
+      table_action NoAction_body.
+      { entailer. }
+      { apply arg_ret_implies_refl. }
+    }
+    { reflexivity. }
+    { reflexivity. }
+    simpl_assertion.
+    entailer.
+  }
+  destruct (get_clear_frame new_timer =? 3) eqn:?.
+  { replace (get_clear_frame new_timer) with 3 by lia.
+    step_call verif_Win1.Win_body _ _ is.
+    { entailer. }
+    { solve [repeat constructor]. }
+    { auto. }
+    step_call verif_Win2.Win_body _ _ is.
+    { entailer. }
+    { solve [repeat constructor]. }
+    { auto. }
+    step_call verif_Win3.Win_body _ _ is.
+    { entailer. }
+    { solve [repeat constructor]. }
+    { auto. }
+    simpl Z.eqb. cbn match.
+    step_call tbl_merge_wins_1_body.
+    { entailer. }
+    { reflexivity. }
+    { reflexivity. }
+    Intros _.
+    simpl_assertion.
+    step_into.
+    { hoare_func_table; elim_trivial_cases.
+      { clear -H5; lia. }
+      table_action NoAction_body.
+      { entailer. }
+      { apply arg_ret_implies_refl. }
+    }
+    { reflexivity. }
+    { reflexivity. }
+    simpl_assertion.
+    entailer.
+  }
+  lia.
+Time Qed.
