examples/cms/verif_CMS_query.v
@@ -1,0 +1,493 @@
+Require Import Poulet4.P4light.Syntax.P4defs.
+Require Import Poulet4.P4light.Semantics.Semantics.
+Require Import ProD3.core.Core.
+Require Import ProD3.core.Tofino.
+Require Import ProD3.examples.cms.ConModel.
+Require Import ProD3.examples.cms.common.
+Require Import ProD3.examples.cms.ModelRepr.
+Require Import ProD3.examples.cms.verif_Win1.
+Require Import ProD3.examples.cms.verif_Win2.
+Require Import ProD3.examples.cms.verif_Win3.
+Require Import ProD3.examples.cms.verif_CMS_1.
+
+#[local] Hint Extern 5 (func_modifies _ _ _ _ _) => (apply tbl_hash_index_1_body) : func_specs.
+#[local] Hint Extern 5 (func_modifies _ _ _ _ _) => (apply tbl_hash_index_2_body) : func_specs.
+#[local] Hint Extern 5 (func_modifies _ _ _ _ _) => (apply tbl_hash_index_3_body) : func_specs.
+#[local] Hint Extern 5 (func_modifies _ _ _ _ _) => (apply tbl_hash_index_4_body) : func_specs.
+#[local] Hint Extern 5 (func_modifies _ _ _ _ _) => (apply tbl_hash_index_5_body) : func_specs.
+#[local] Hint Extern 5 (func_modifies _ _ _ _ _) => (apply tbl_clear_index_body) : func_specs.
+#[local] Hint Extern 5 (func_modifies _ _ _ _ _) => (apply tbl_clear_window_body) : func_specs.
+#[local] Hint Extern 5 (func_modifies _ _ _ _ _) => (apply act_set_clear_win_1_body) : func_specs.
+#[local] Hint Extern 5 (func_modifies _ _ _ _ _) => (apply act_set_clear_win_2_body) : func_specs.
+#[local] Hint Extern 5 (func_modifies _ _ _ _ _) => (apply act_set_clear_win_3_body) : func_specs.
+
+Definition P4_bf2_win_md_t_query (f cf if' : Z) (new_clear_index : Sval) (is : list Sval) :=
+  if f=? cf then
+    P4_bf2_win_md_t (P4Bit 8 CLEAR) (Zrepeat new_clear_index 5)
+  else
+    P4_bf2_win_md_t (P4Bit 8 QUERY) is.
+
+Definition tbl_set_win_query_spec : func_spec :=
+  WITH (* p *),
+    PATH p
+    MOD (Some [["ds_md"];
+               ["act_set_clear_win_1"; "api_1"];
+               ["act_set_clear_win_1"; "api_2"];
+               ["act_set_clear_win_1"; "api_3"];
+               ["act_set_clear_win_2"; "api_1"];
+               ["act_set_clear_win_2"; "api_2"];
+               ["act_set_clear_win_2"; "api_3"];
+               ["act_set_clear_win_3"; "api_1"];
+               ["act_set_clear_win_3"; "api_2"];
+               ["act_set_clear_win_3"; "api_3"];
+               ["act_set_clear_win_4"; "api_1"];
+               ["act_set_clear_win_4"; "api_2"];
+               ["act_set_clear_win_4"; "api_3"];
+               ["act_set_clear_win_5"; "api_1"];
+               ["act_set_clear_win_5"; "api_2"];
+               ["act_set_clear_win_5"; "api_3"]]) []
+    WITH (timer : Z * bool) (clear_index_1 hash_index_1 hash_index_2 hash_index_3 hash_index_4 hash_index_5 : Sval)
+      (H_timer : 0 <= fst timer < frame_tick_tocks * num_frames),
+      PRE
+        (ARG []
+        (MEM [(["api"], P4Bit 8 QUERY);
+              (["ds_md"], ValBaseStruct
+                 [("clear_window", P4Bit 16 (fst timer));
+                  ("clear_index_1", clear_index_1);
+                  ("hash_index_1", hash_index_1);
+                  ("hash_index_2", hash_index_2);
+                  ("hash_index_3", hash_index_3);
+                  ("hash_index_4", hash_index_4);
+                  ("hash_index_5", hash_index_5);
+                  ("win_1", P4_bf2_win_md_t_);
+                  ("win_2", P4_bf2_win_md_t_);
+                  ("win_3", P4_bf2_win_md_t_)])]
+        (EXT [])))
+      POST
+        (EX retv,
+        (ARG_RET [] retv
+        (let cf := get_clear_frame timer in
+        let if' := get_insert_frame cf in
+        (MEM [(["ds_md"], ValBaseStruct
+                 [("clear_window", P4Bit 16 (fst timer));
+                  ("clear_index_1", clear_index_1);
+                  ("hash_index_1", hash_index_1);
+                  ("hash_index_2", hash_index_2);
+                  ("hash_index_3", hash_index_3);
+                  ("hash_index_4", hash_index_4);
+                  ("hash_index_5", hash_index_5);
+                  ("win_1", P4_bf2_win_md_t_query 0 cf if' clear_index_1
+                        [hash_index_1; hash_index_2; hash_index_3; hash_index_4; hash_index_5]);
+                  ("win_2", P4_bf2_win_md_t_query 1 cf if' clear_index_1
+                        [hash_index_1; hash_index_2; hash_index_3; hash_index_4; hash_index_5]);
+                  ("win_3", P4_bf2_win_md_t_query 2 cf if' clear_index_1
+                        [hash_index_1; hash_index_2; hash_index_3; hash_index_4; hash_index_5])])]
+        (EXT [])))))%arg_ret_assr.
+
+Lemma tbl_set_win_query_body :
+  func_sound ge tbl_set_win_fd nil tbl_set_win_query_spec.
+Proof.
+  start_function; elim_trivial_cases.
+  - replace (get_clear_frame timer) with 0. 2 : {
+      symmetry; eapply Z_div_squeeze'; eauto.
+    }
+    table_action act_set_clear_win_1_body.
+    { entailer. }
+    { entailer. }
+  - replace (get_clear_frame timer) with 1. 2 : {
+      symmetry; eapply Z_div_squeeze'; eauto.
+    }
+    table_action act_set_clear_win_2_body.
+    { entailer. }
+    { entailer. }
+  - replace (get_clear_frame timer) with 2. 2 : {
+      symmetry; eapply Z_div_squeeze'; eauto.
+    }
+    table_action act_set_clear_win_3_body.
+    { entailer. }
+    { entailer. }
+  - lia.
+Qed.
+
+(* Definition act_merge_wins_fd :=
+  ltac:(get_fd ["Bf2BloomFilter"; "act_merge_wins"] ge).
+
+Definition act_merge_wins_spec : func_spec :=
+  WITH (* p *),
+    PATH p
+    MOD (Some [["query_res"]]) []
+    WITH,
+      PRE
+        (ARG []
+        (MEM []
+        (EXT [])))
+      POST
+        (ARG_RET [] ValBaseNull
+        (MEM [(["query_res"], (P4Bit 8 1))]
+        (EXT []))).
+
+Lemma act_merge_wins_body :
+  func_sound ge act_merge_wins_fd nil act_merge_wins_spec.
+Proof.
+  start_function.
+  step.
+  step.
+  entailer.
+Qed.
+
+Definition act_merge_default_fd :=
+  ltac:(get_fd ["Bf2BloomFilter"; "act_merge_default"] ge).
+
+Definition act_merge_default_spec : func_spec :=
+  WITH (* p *),
+    PATH p
+    MOD (Some [["query_res"]]) []
+    WITH,
+      PRE
+        (ARG []
+        (MEM []
+        (EXT [])))
+      POST
+        (ARG_RET [] ValBaseNull
+        (MEM [(["query_res"], (P4Bit 8 0))]
+        (EXT []))).
+
+Lemma act_merge_default_body :
+  func_sound ge act_merge_default_fd nil act_merge_default_spec.
+Proof.
+  start_function.
+  step.
+  step.
+  entailer.
+Qed. *)
+
+(* Definition tbl_merge_wins_fd :=
+  ltac:(get_fd ["Bf2BloomFilter"; "tbl_merge_wins"; "apply"] ge). *)
+
+Definition tbl_merge_wins_final_spec : func_spec :=
+  WITH (* p *),
+    PATH p
+    MOD (Some [["query_res"]]) []
+    WITH ds_md,
+      PRE
+        (ARG []
+        (MEM [(["api"], P4Bit 8 QUERY);
+              (["ds_md"], ds_md)]
+        (EXT [])))
+      POST
+        (EX retv,
+        (ARG_RET [] retv
+        (MEM [(["query_res"], abs_plus_sat
+          (get "rw_1" (get "win_1" ds_md))
+          (get "rw_1" (get "win_2" ds_md)))]
+        (EXT []))))%arg_ret_assr.
+
+Lemma tbl_merge_wins_final_body :
+  func_sound ge tbl_merge_wins_final_fd nil tbl_merge_wins_final_spec.
+Proof.
+  start_function; elim_trivial_cases.
+  2 : lia.
+  table_action act_merge_wins_final_body.
+  { entailer. }
+  { reflexivity. }
+  { reflexivity. }
+  { entailer. }
+Qed.
+
+#[local] Instance Inhabitant_ext_pred : Inhabitant ext_pred :=
+  ExtPred.prop True.
+
+Lemma ext_implies_ext : forall a1 a2,
+  Zlength a1 = Zlength a2 ->
+  (forall i, 0 <= i < Zlength a1 -> ext_implies [Znth i a1] [Znth i a2]) ->
+  ext_implies a1 a2.
+Proof.
+Admitted.
+
+Require Import ProD3.examples.sbf.Utils.
+
+Lemma frame_query_bound : forall p (* rows *) (cf : frame) is,
+  (* Zlength rows = num_rows -> *)
+  Zlength is = num_rows ->
+  Forall (fun i : Z => 0 <= i < num_slots) is ->
+  ext_implies [frame_repr p rows cf] [ExtPred.prop (frame_query cf is >= 0)].
+Proof.
+  intros.
+  assert (Zlength rows = num_rows) by auto.
+  unfold frame_repr, frame_query.
+  rewrite ext_pred_wrap_cons.
+  eapply ext_implies_trans with (map2 (fun cr i => ExtPred.prop (row_query cr i >= 0)) (proj1_sig cf) is).
+  - destruct cf as [crs ?].
+    cbn [proj1_sig].
+    apply ext_implies_ext.
+    { list_solve. }
+    intros.
+    list_simplify.
+    do 2 rewrite Znth_map2 by list_solve.
+    apply row_query_bound; list_solve.
+  - (* 
+      list_solve.
+  generalize dependent cf.
+  
+  destruct cr as [cr ?H]. unfold row_query. cbn [proj1_sig].
+  normalize_EXT.
+  Intros_prop.
+  apply ext_implies_prop_intro.
+  list_solve. *)
+(* Qed. *)
+Admitted.
+
+Definition cms_query := @cms_query num_frames num_rows num_slots H_num_frames H_num_rows H_num_slots
+  frame_tick_tocks.
+
+Definition Filter_query_spec : func_spec :=
+  WITH (* p *),
+    PATH p
+    MOD None [p]
+    WITH (key : Val) (tstamp : Z) (cf : cms num_frames num_rows num_slots),
+      PRE
+        (ARG [eval_val_to_sval key; P4Bit 8 QUERY; P4Bit 48 tstamp; P4Bit_ 8]
+        (MEM []
+        (EXT [cms_repr p index_w panes rows cf])))
+      POST
+        (ARG_RET [P4Bit value_w (Z.min (
+          snd (cms_query cf (Z.odd (tstamp/tick_time)) (hashes key)))
+          (2 ^ 32 -1))] ValBaseNull
+        (MEM []
+        (EXT [cms_repr p index_w panes rows (fst (cms_query cf (Z.odd (tstamp/tick_time)) (hashes key)))]))).
+
+Ltac destruct_listn l :=
+  destruct l as [l ?H];
+  destruct_list l.
+
+Lemma Filter_query_body :
+  func_sound ge Filter_fd nil Filter_query_spec.
+Proof.
+  start_function.
+  destruct cf as [[ps ?H] ? ?].
+  unfold cms_repr.
+  cbn [proj1_sig] in *.
+  destruct_list ps.
+  normalize_EXT.
+  step.
+  step_call tbl_hash_index_1_body.
+  { entailer. }
+  Intros _.
+  step_call tbl_hash_index_2_body.
+  { entailer. }
+  Intros _.
+  step_call tbl_hash_index_3_body.
+  { entailer. }
+  Intros _.
+  step_call tbl_hash_index_4_body.
+  { entailer. }
+  Intros _.
+  step_call tbl_hash_index_5_body.
+  { entailer. }
+  Intros _.
+  set (is := (exist _ [hash1 key; hash2 key; hash3 key; hash4 key; hash5 key] eq_refl : listn Z 5)).
+  set (clear_is := (exist _ (Zrepeat cms_clear_index 5) eq_refl : listn Z 5)).
+  assert (Forall (fun i : Z => 0 <= i < num_slots) (`is)). {
+    repeat first [apply Forall_cons | apply Forall_nil].
+    all : unfold hash1, hash2, hash3;
+      apply Z.mod_pos_bound; lia.
+  }
+  P4assert (0 <= cms_clear_index < num_slots). {
+    unfold fil_clear_index_repr.
+    Intros i'.
+    normalize_EXT.
+    Intros_prop.
+    apply ext_implies_prop_intro.
+    subst.
+    apply Z.mod_pos_bound.
+    lia.
+  }
+  assert (Forall (fun i : Z => 0 <= i < num_slots) (`clear_is)). {
+    repeat first [
+      assumption
+    | constructor
+    ].
+  }
+  step_call tbl_clear_index_body.
+  { entailer. }
+  Intros _.
+  step_call tbl_clear_window_body.
+  { entailer. }
+  Intros _.
+  set (new_timer := update_timer cms_timer (Z.odd (tstamp / tick_time))).
+  P4assert (0 <= fst new_timer < num_frames * frame_tick_tocks).
+  { unfold timer_repr.
+    normalize_EXT.
+    Intros_prop.
+    apply ext_implies_prop_intro.
+    auto.
+  }
+  step_call tbl_set_win_query_body.
+  { entailer. }
+  { auto. }
+  Intros _.
+  (* unfold and fold in the post condition *)
+  unfold cms_query, ConModel.cms_query.
+  (* cbn [proj1_sig fst snd]. *)
+  unfold proj1_sig. unfold fst. unfold snd.
+  fold new_timer.
+  replace (exist (fun i : list Z => Zlength i = num_rows) (Zrepeat cms_clear_index num_rows) _) with clear_is. 2 : {
+    apply subset_eq_compat. auto.
+  }
+  assert (0 <= get_clear_frame new_timer < num_frames). {
+    unfold ConModel.get_clear_frame.
+    split.
+    - apply Z.div_le_lower_bound; lia.
+    - apply Z.div_lt_upper_bound; lia.
+  }
+
+Ltac pose_frame_query_bound f is :=
+  P4assert (frame_query f (`is) >= 0);
+  only 1 : (
+    eapply ext_implies_trans;
+    only 2 : (apply frame_query_bound; auto);
+    entailer
+  ).
+
+  pose_frame_query_bound x is.
+  pose_frame_query_bound x0 is.
+  pose_frame_query_bound x1 is.
+
+  destruct (get_clear_frame new_timer =? 0) eqn:?.
+  { replace (get_clear_frame new_timer) with 0 by lia.
+    step_call verif_Win1.Win_body _ _ clear_is.
+    { entailer. }
+    { solve [repeat constructor]. }
+    { auto. }
+    step_call verif_Win2.Win_body _ _ is.
+    { entailer. }
+    { solve [repeat constructor]. }
+    { auto. }
+    step_call verif_Win3.Win_body _ _ is.
+    { entailer. }
+    { solve [repeat constructor]. }
+    { auto. }
+    simpl Z.eqb. cbn match.
+    step_call tbl_merge_wins_1_body.
+    { entailer. }
+    { reflexivity. }
+    { reflexivity. }
+    Intros _.
+    simpl_assertion.
+    step_into.
+    { hoare_func_table; elim_trivial_cases.
+      2 : { clear -H8; lia. }
+      table_action act_merge_wins_final_body.
+      { entailer. }
+      { reflexivity. }
+      { reflexivity. }
+      { apply arg_ret_implies_refl. }
+    }
+    { reflexivity. }
+    { reflexivity. }
+    entailer.
+    simpl_assertion.
+    repeat rewrite abs_plus_sat_bit.
+    repeat rewrite sat_bound_spec.
+    unfold value_w.
+    rewrite_strat bottomup mod_bound_small.
+    2-5 : lia.
+    apply sval_refine_refl'. f_equal.
+    unfold Zsum, fold_left. simpl.
+    change ([hash1 key; hash2 key; hash3 key; hash4 key; hash5 key])
+      with (`is).
+    lia.
+  }
+  destruct (get_clear_frame new_timer =? 1) eqn:?.
+  { replace (get_clear_frame new_timer) with 1 by lia.
+    step_call verif_Win1.Win_body _ _ is.
+    { entailer. }
+    { solve [repeat constructor]. }
+    { auto. }
+    step_call verif_Win2.Win_body _ _ clear_is.
+    { entailer. }
+    { solve [repeat constructor]. }
+    { auto. }
+    step_call verif_Win3.Win_body _ _ is.
+    { entailer. }
+    { solve [repeat constructor]. }
+    { auto. }
+    simpl Z.eqb. cbn match.
+    step_call tbl_merge_wins_1_body.
+    { entailer. }
+    { reflexivity. }
+    { reflexivity. }
+    Intros _.
+    simpl_assertion.
+    step_into.
+    { hoare_func_table; elim_trivial_cases.
+      2 : { clear -H8; lia. }
+      table_action act_merge_wins_final_body.
+      { entailer. }
+      { reflexivity. }
+      { reflexivity. }
+      { apply arg_ret_implies_refl. }
+    }
+    { reflexivity. }
+    { reflexivity. }
+    entailer.
+    simpl_assertion.
+    repeat rewrite abs_plus_sat_bit.
+    repeat rewrite sat_bound_spec.
+    unfold value_w.
+    rewrite_strat bottomup mod_bound_small.
+    2-5 : lia.
+    apply sval_refine_refl'. f_equal.
+    unfold Zsum, fold_left. simpl.
+    change ([hash1 key; hash2 key; hash3 key; hash4 key; hash5 key])
+      with (`is).
+    lia.
+  }
+  destruct (get_clear_frame new_timer =? 2) eqn:?.
+  { replace (get_clear_frame new_timer) with 2 by lia.
+    step_call verif_Win1.Win_body _ _ is.
+    { entailer. }
+    { solve [repeat constructor]. }
+    { auto. }
+    step_call verif_Win2.Win_body _ _ is.
+    { entailer. }
+    { solve [repeat constructor]. }
+    { auto. }
+    step_call verif_Win3.Win_body _ _ clear_is.
+    { entailer. }
+    { solve [repeat constructor]. }
+    { auto. }
+    simpl Z.eqb. cbn match.
+    step_call tbl_merge_wins_1_body.
+    { entailer. }
+    { reflexivity. }
+    { reflexivity. }
+    Intros _.
+    simpl_assertion.
+    step_into.
+    { hoare_func_table; elim_trivial_cases.
+      2 : { clear -H8; lia. }
+      table_action act_merge_wins_final_body.
+      { entailer. }
+      { reflexivity. }
+      { reflexivity. }
+      { apply arg_ret_implies_refl. }
+    }
+    { reflexivity. }
+    { reflexivity. }
+    entailer.
+    simpl_assertion.
+    repeat rewrite abs_plus_sat_bit.
+    repeat rewrite sat_bound_spec.
+    unfold value_w.
+    rewrite_strat bottomup mod_bound_small.
+    2-5 : lia.
+    apply sval_refine_refl'. f_equal.
+    unfold Zsum, fold_left. simpl.
+    change ([hash1 key; hash2 key; hash3 key; hash4 key; hash5 key])
+      with (`is).
+    lia.
+  }
+  lia.
+(* This is slow. I can understand it but I don't know the direct reason. *)
+Qed.
